Tests/Equiv.lean
@@ -1,0 +1,23 @@
+import Quotify.Command
+
+@[quotify]
+def s₁ : Setoid (List α) where
+  r := List.Perm
+  iseqv := sorry
+
+/-- info: ✅ -/
+#guard_msgs in
+#quotify_equiv List.Perm
+
+/-- info: ❌ -/
+#guard_msgs in
+#quotify_equiv @List.Perm Nat
+
+@[quotify]
+def s₂ : Setoid (List Nat) where
+  r := List.Perm
+  iseqv := sorry
+
+/-- info: ✅ -/
+#guard_msgs in
+#quotify_equiv @List.Perm Nat
