Tests/Norm.lean
@@ -1,0 +1,51 @@
+import Quotify.Command
+
+set_option pp.explicit true
+
+/-- info: [0] @List.Perm Nat -/
+#guard_msgs in
+#quotify_norm @List.Perm Nat
+
+/-- info: [0] @List.Perm Nat -/
+#guard_msgs in
+#quotify_norm ((· ≈ ·) : List Nat → List Nat → Prop)
+
+/-- info: [1] fun x_0 => @List.Perm x_0 -/
+#guard_msgs in
+#quotify_norm List.Perm
+
+/-- info: [1] fun x_0 => @List.Perm x_0 -/
+#guard_msgs in
+#quotify_norm (List.isSetoid _).r
+
+/-- info: [1] fun α => @List.Perm α -/
+#guard_msgs in
+#quotify_norm ((· ≈ ·) : List ?α → List ?α → Prop)
+
+/-- info: [1] fun x_0 l₁ l₂ => ∀ (x : x_0), Iff (@List.Mem x_0 x l₁) (@List.Mem x_0 x l₂) -/
+#guard_msgs in
+#quotify_norm fun α (l₁ l₂ : List α) => ∀ x, x ∈ l₁ ↔ x ∈ l₂
+
+/-- info: [1] fun x_0 => @Eq x_0 -/
+#guard_msgs in
+#quotify_norm (· = ·)
+
+opaque MyEquiv₁ : Bool → Bool → Prop
+
+/-- info: [0] MyEquiv₁ -/
+#guard_msgs in
+#quotify_norm MyEquiv₁
+
+def MyEquiv₂ (b₁ b₂ : Bool) : Prop :=
+  b₁ = b₂
+
+/-- info: [0] MyEquiv₂ -/
+#guard_msgs in
+#quotify_norm MyEquiv₂
+
+abbrev MyEquiv₃ (b₁ b₂ : Bool) : Prop :=
+  b₁ = b₂
+
+/-- info: [0] @Eq Bool -/
+#guard_msgs in
+#quotify_norm MyEquiv₃
