Tests/Quot.lean
@@ -1,0 +1,18 @@
+import Quotify.Command
+
+attribute [quotify] List.isSetoid
+
+/--
+info: fun x_0 lhs rhs => Quotient.mk { r := List.Perm, iseqv := ⋯ } lhs = Quotient.mk { r := List.Perm, iseqv := ⋯ } rhs
+-/
+#guard_msgs in
+#quotify_quot List.Perm
+
+/--
+info: fun α lhs rhs => Quotient.mk { r := List.Perm, iseqv := ⋯ } lhs = Quotient.mk { r := List.Perm, iseqv := ⋯ } rhs
+-/
+#guard_msgs in
+#quotify_quot ((· ≈ ·) : List ?α → List ?α → Prop)
+
+-- TODO
+#quotify_quot @List.Perm Nat
