Tests/Setoid.lean
@@ -1,0 +1,37 @@
+import Quotify.Command
+
+@[quotify]
+def s₁ : Setoid (List α) where
+  r := List.Perm
+  iseqv := sorry
+
+/--
+error: There already exists a `Setoid` marked with `[quotify]` for the relation ⏎
+  fun x_0 => List.Perm
+-/
+#guard_msgs(error) in
+@[quotify]
+def s₂ : Setoid (List α) where
+  r := List.Perm
+  iseqv := sorry
+
+-- The relation here is `fun x_0 => @Setoid.r (List x_0) (@s₁ x_0)`.
+@[quotify]
+def s₃ : Setoid (List α) where
+  r := s₁.r
+  iseqv := sorry
+
+-- TODO: Shouldn't the relation reduce to the same as `s₃`? Note, I think we can afford to use
+--       normalized relations only as the fast path, but check for definitional equality as well.
+-- The relation here is `fun x_0 => @Setoid.r (List x_0) ((@fun {α} => (@fun {α} => @s₁ α) α) x_0)`.
+@[quotify]
+def s₄ : Setoid (List α) := s₁
+
+/--
+error: There already exists a `Setoid` marked with `[quotify]` for the relation ⏎
+  fun x_0 => List.Perm
+-/
+#guard_msgs in
+attribute [instance] s₁ in
+@[quotify]
+def s₅ : Setoid (List α) := s₁
