Tests/Theorems.lean
@@ -1,0 +1,46 @@
+import Quotify.Command
+
+@[quotify]
+theorem t₁ : [].Perm (α := α) [] := by rfl
+
+@[quotify]
+theorem t₂ (l₁ l₂ : List α) : l₁ ≈ l₂ := sorry
+
+@[quotify]
+theorem t₃ (l₁ l₂ : List α) : (List.isSetoid _).r l₁ l₂ := sorry
+
+/-- info: [t₁, t₂, t₃] -/
+#guard_msgs in
+#quotify_theorems List.Perm
+
+namespace X
+
+opaque t₁ : Nat
+
+/-- info: [_root_.t₁, t₂, t₃] -/
+#guard_msgs in
+#quotify_theorems List.Perm
+
+end X
+
+@[quotify]
+theorem t₄ (l₁ l₂ : List Nat) : l₁ ≈ l₂ := sorry
+
+/-- info: [t₁, t₂, t₃] -/
+#guard_msgs in
+#quotify_theorems List.Perm
+
+/-- info: [t₄] -/
+#guard_msgs in
+#quotify_theorems @List.Perm Nat
+
+/--
+info: fun α => @List.Perm α:
+[t₁, t₂, t₃]
+---
+info: @List.Perm Nat:
+[t₄]
+-/
+#guard_msgs in
+set_option pp.explicit true in
+#quotify_theorems
